Equiv/SimF.v
@@ -50,20 +50,20 @@ Qed.
 Definition simLabenv t (r:frel)
            {A} (PR:ProofRelation A) (AL:list A) L L' :=
   (length AL = length L /\ sawtooth L' /\ sawtooth L) /\
-  forall f f' a Z s n Z' s' n' V V',
-    IndexRel AL f f'
-    -> get AL f a
-    -> get L f (F.blockI V Z s n)
-    -> get L' f' (F.blockI V' Z' s' n')
+  forall f f' a V Z s n V' Z' s' n',
+    IndexRel AL (counted f) (counted f')
+    -> get AL (counted f) a
+    -> get L (counted f) (F.blockI V Z s n)
+    -> get L' (counted f') (F.blockI V' Z' s' n')
     -> (ParamRel a Z Z' /\ BlockRel a (F.blockI V Z s n) (F.blockI V' Z' s' n'))
       /\ (forall E E' Yv Y'v Y Y',
             ArgRel a Yv Y'v
             -> omap (exp_eval E) Y = Some Yv
             -> omap (exp_eval E') Y' = Some Y'v
-            -> sim'r r t (drop (f  - n) L, E, stmtApp (LabI n) Y)
-                    (drop (f'  - n') L', E', stmtApp (LabI n') Y')).
+            -> sim'r r t (L, E, stmtApp f Y)
+                    (L', E', stmtApp f' Y')).
 
-Lemma simILabenv_mon t (r r':frel) A (PR:ProofRelation A) AL L L'
+Lemma simLabenv_mon t (r r':frel) A (PR:ProofRelation A) AL L L'
   : simLabenv t r PR AL L L'
     -> (forall t x y, r t x y -> r' t x y)
     -> simLabenv t r' PR AL L L'.
@@ -82,7 +82,30 @@ Definition indexwise_proofrel A (PR:ProofRelation A) E E' (F F':〔params * stmt
     -> get AL' n a
     -> ParamRel a Z Z' /\ BlockRel a (F.blockI E Z s n) (F.blockI E' Z' s' n').
 
-Lemma simILabenv_extension' t (r:frel) A (PR:ProofRelation A) (AL AL':list A) E E' F F' L L'
+
+Lemma stepGoto_mapi L blk Y E vl f F V
+      (Ldef:get L (counted f - ❬F❭) blk)
+      (len:length (F.block_Z blk) = length Y)
+      (def:omap (exp_eval V) Y = Some vl) E'
+      (updOk:F.block_E blk [F.block_Z blk <-- List.map Some vl] = E')
+      (ST:sawtooth L) (GE: counted f >= ❬F❭)
+  : F.step (mapi (F.mkBlock E) F ++ L, V, stmtApp f Y) EvtTau
+           (drop (counted f - ❬F❭ - block_n blk) L,
+            E', F.block_s blk).
+Proof.
+  rewrite <- (mapi_length (F.mkBlock E)).
+  assert (counted f - block_n blk >= ❬mapi (F.mkBlock E) F❭). {
+    exploit (sawtooth_smaller ST Ldef).
+    rewrite mapi_length. simpl in *. omega.
+  }
+  orewrite (counted f - ❬mapi (F.mkBlock E) F❭ - block_n blk
+            =  (counted f - block_n blk) - ❬mapi (F.mkBlock E) F❭).
+  rewrite <- (drop_app_gen _ (mapi (F.mkBlock E) F)); eauto.
+  eapply F.stepGoto; eauto.
+  rewrite get_app_ge. rewrite mapi_length. eauto. omega.
+Qed.
+
+Lemma simLabenv_extension' t (r:frel) A (PR:ProofRelation A) (AL AL':list A) E E' F F' L L'
       (LEN1:length AL' = length F)
   : indexwise_r t (sim'r r \3/ r) PR AL' E E' F F' AL L L'
     -> indexwise_proofrel PR E E' F F' AL' AL
@@ -99,51 +122,43 @@ Proof.
   destruct SIML; dcr; split; eauto with len. split; eauto.
   econstructor; eauto. eapply tooth_F_mkBlocks.
   econstructor; eauto. eapply tooth_F_mkBlocks.
-  intros ? ? ? ? ? ? ? ? ? V V' RN GetAL GetFL GetL'.
+  intros f f' ? ? ? ? ? ? ? ? ? RN GetAL GetFL GetL'.
   assert (❬AL'❭ = ❬mapi (F.mkBlock E) F❭) by eauto with len.
   eapply get_app_cases in GetAL. destruct GetAL as [GetAL'|GetAL].
   - eapply get_app_lt_1 in GetFL; [| rewrite <- H; eauto using get_range].
     inv_get. destruct x as [Z s]. simpl in *. clear EQ.
-    orewrite (n - n = 0). simpl.
     exploit Ilt; eauto using get_range.
     eapply get_app_lt_1 in GetL'; [| rewrite mapi_length; eauto with len ].
     inv_get. destruct x as [Z' s']; simpl in *; clear EQ.
     split; eauto.
     intros.
     exploit (ArgLengthMatchI); eauto; dcr. eapply IP; eauto.
-    exploit (omap_length _ _ _ _ _ H2).
-    exploit (omap_length _ _ _ _ _ H3).
-    pone_step; eauto using get_app, get_mapi; eauto; simpl; try congruence.
-    orewrite (n' - n' = 0); simpl.
-    eapply get_app. eapply mapi_get_1; eauto.
-    simpl. congruence.
-    orewrite (n - n = 0); simpl.
-    orewrite (n' - n' = 0); simpl.
+    pone_step; eauto using get_app, get_mapi; eauto; simpl; eauto with len.
+    orewrite (labN f - labN f = 0); simpl.
+    orewrite (labN f' - labN f' = 0); simpl.
     eapply ISIM; eauto.
   - destruct SIML; dcr.
     eapply get_app_right_ge in GetFL; [ | rewrite <- H; eauto].
     exploit Ige; eauto; try congruence.
-    eapply get_app_right_ge in GetL'; [ | eauto with len; rewrite mapi_length; eauto].
-    rewrite mapi_length in *.
+    eapply get_app_right_ge in GetL'; [ | eauto with len; rewrite mapi_length; eauto].    rewrite mapi_length in *.
     eapply IndexRelDrop in RN; eauto.
-    edestruct H1 as [[? ?] SIM]; eauto. rewrite H; eauto. rewrite Img; eauto.
+    edestruct (H1 (LabI (counted f - ❬AL'❭)) (LabI (counted f' - Image AL')))
+      as [[? ?] SIM]; simpl; eauto.
+    rewrite H; eauto. rewrite Img; eauto.
     split; eauto.
     intros.
-    assert (f - n >= ❬mapi (F.mkBlock E) F❭). {
-      exploit (sawtooth_smaller H7 GetFL).
-      rewrite <- H in *. rewrite mapi_length. simpl in *. omega.
-    }
-    assert (f' - n' >= ❬mapi (F.mkBlock E') F'❭). {
-      exploit (sawtooth_smaller H6 GetL').
-      rewrite mapi_length in *.
-      simpl in *. omega.
-    }
-    rewrite (drop_app_gen _ (mapi (F.mkBlock E) F)); eauto.
-    rewrite (drop_app_gen _ (mapi (F.mkBlock E') F')); eauto.
-    repeat rewrite mapi_length. rewrite H in SIM. rewrite Img in SIM.
-    orewrite (f - n - ❬F❭ = f - ❬F❭ - n).
-    orewrite (f' - n' - ❬F'❭ = f' - ❬F'❭ - n').
-    eapply paco3_mon. eapply SIM; eauto. eauto.
+    exploit (ArgLengthMatchI); eauto; dcr.
+    eapply (@sim_Y_left F.state _ F.state _).
+    eapply (@sim_Y_right F.state _ F.state _).
+    rewrite Img in SIM. rewrite H in SIM.
+    eapply SIM; eauto.
+    econstructor; simpl; eauto with len. simpl. eauto with len.
+    Focus 2.
+    econstructor; simpl; eauto. simpl. eauto with len.
+    simpl.
+    eapply (stepGoto_mapi _ _ _ _ _ GetL'); simpl; eauto with len.
+    eapply (stepGoto_mapi _ _ _ _ _ GetFL); simpl; eauto with len.
+    simpl in *; omega.
 Qed.
 
 Lemma fix_compatible_I t A (PR:ProofRelation A) AL F F' E E' L L' AL'
@@ -164,7 +179,7 @@ Proof.
   destruct SIML; dcr; split; eauto with len. split.
   econstructor; eauto. eapply tooth_F_mkBlocks.
   econstructor; eauto. eapply tooth_F_mkBlocks.
-  eapply simILabenv_extension'; eauto using simILabenv_mon, indexwise_r_mon.
+  eapply simLabenv_extension'; eauto using simLabenv_mon, indexwise_r_mon.
 Qed.
 
 Lemma simILabenv_extension t A (PR:ProofRelation A) (AL AL':list A) E E' F F' L L'
@@ -181,12 +196,13 @@ Lemma simILabenv_extension t A (PR:ProofRelation A) (AL AL':list A) E E' F F' L 
                        (mapi (F.mkBlock E) F ++ L)
                        (mapi (F.mkBlock E') F' ++ L').
 Proof.
-  intros. eapply simILabenv_extension'; eauto.
+  intros. eapply simLabenv_extension'; eauto.
   eapply indexwise_r_mon.
   eapply fix_compatible_I; eauto. eauto.
 Qed.
 
-Lemma renILabenv_extension_len t A (PR:ProofRelation A) (AL AL':list A) E E' F F' L L'
+Lemma simLabenv_extension_len t A (PR:ProofRelation A) (AL AL':list A)
+      E E' F F' L L'
       (LEN1:length AL' = length F) (LEN2:length F = length F')
       (IDX:forall AL n n', IndexRel AL n n' = (n = n'))
   : (forall r, simLabenv t r PR (AL' ++ AL) (mapi (F.mkBlock E) F ++ L)
@@ -203,7 +219,7 @@ Proof.
   intros. rewrite IDX in H. subst; omega.
   assert (forall n n', IndexRel (AL' ++ AL) n n' -> n >= length F -> n' >= length F').
   intros. rewrite IDX in H0. subst; omega.
-  intros. eapply simILabenv_extension'; eauto.
+  intros. eapply simLabenv_extension'; eauto.
   eapply indexwise_r_mon.
   eapply fix_compatible_I; eauto. eauto.
 Qed.
